add algorithm and start proving theorems

src/SSA2QFBV.v
@@ -4,9 +4,427 @@ From mathcomp Require Import ssreflect ssrnat ssrbool eqtype seq ssrfun.
 From ssrlib Require Import Var.
 From BitBlasting Require Import State QFBV.
 From Cryptoline Require Import DSL SSA.
+From nbits Require Import NBits. 
 
 Import SSA.
+
+Set Implicit Arguments.
+Unset Strict Implicit.
+Import Prenex Implicits.
+
+Definition qfbv_atomic a :=
+  match a with
+  | SSA.Avar v => QFBV.Evar v
+  | SSA.Aconst ty n => QFBV.Econst n
+  end .
+
+Definition qfbv_var v := QFBV.Evar v .
+
+Definition qfbv_const n := QFBV.Econst (NBitsDef.from_nat n n) .
+
+Definition qfbv_zero w := QFBV.Econst (NBitsDef.from_nat w 0) .
+
+Definition qfbv_one w := QFBV.Econst (NBitsDef.from_nat w 1) .
+
+Definition qfbv_not qe := QFBV.Eunop QFBV.Unot qe .
+
+Definition qfbv_neg qe := QFBV.Eunop QFBV.Uneg qe .
+
+Definition qfbv_extr i j qe := QFBV.Eunop (QFBV.Uextr i j) qe .
+
+Definition qfbv_high n qe := QFBV.Eunop (QFBV.Uhigh n) qe .
+
+Definition qfbv_low n qe := QFBV.Eunop (QFBV.Ulow n) qe .
+
+Definition qfbv_zext n qe := QFBV.Eunop (QFBV.Uzext n) qe .
+
+Definition qfbv_sext n qe := QFBV.Eunop (QFBV.Usext n) qe .
+
+Definition qfbv_and qe0 qe1 := QFBV.Ebinop QFBV.Band qe0 qe1 .
+
+Definition qfbv_or qe0 qe1 := QFBV.Ebinop QFBV.Bor qe0 qe1 .
+
+Definition qfbv_xor qe0 qe1 := QFBV.Ebinop QFBV.Bxor qe0 qe1 .
+
+Definition qfbv_add qe0 qe1 := QFBV.Ebinop QFBV.Badd qe0 qe1 .
+
+Definition qfbv_sub qe0 qe1 := QFBV.Ebinop QFBV.Bsub qe0 qe1 .
+
+Definition qfbv_mul qe0 qe1 := QFBV.Ebinop QFBV.Bmul qe0 qe1 .
+
+Definition qfbv_mod qe0 qe1 := QFBV.Ebinop QFBV.Bmod qe0 qe1 .
+
+Definition qfbv_srem qe0 qe1 := QFBV.Ebinop QFBV.Bsrem qe0 qe1 .
+
+Definition qfbv_smod qe0 qe1 := QFBV.Ebinop QFBV.Bsmod qe0 qe1 .
+
+Definition qfbv_shl qe0 qe1 := QFBV.Ebinop QFBV.Bshl qe0 qe1 .
+
+Definition qfbv_lshr qe0 qe1 := QFBV.Ebinop QFBV.Blshr qe0 qe1 .
+
+Definition qfbv_ashr qe0 qe1 := QFBV.Ebinop QFBV.Bashr qe0 qe1 .
+
+Definition qfbv_concat qe0 qe1 := QFBV.Ebinop QFBV.Bconcat qe0 qe1 .
+
+Definition qfbv_eq qe0 qe1 := QFBV.Bbinop QFBV.Beq qe0 qe1 .
+
+Definition qfbv_ult qe0 qe1 := QFBV.Bbinop QFBV.Bult qe0 qe1 .
+
+Definition qfbv_ule qe0 qe1 := QFBV.Bbinop QFBV.Bule qe0 qe1 .
+
+Definition qfbv_ugt qe0 qe1 := QFBV.Bbinop QFBV.Bugt qe0 qe1 .
+
+Definition qfbv_uge qe0 qe1 := QFBV.Bbinop QFBV.Buge qe0 qe1 .
+
+Definition qfbv_slt qe0 qe1 := QFBV.Bbinop QFBV.Bslt qe0 qe1 .
+
+Definition qfbv_sle qe0 qe1 := QFBV.Bbinop QFBV.Bsle qe0 qe1 .
+
+Definition qfbv_sgt qe0 qe1 := QFBV.Bbinop QFBV.Bsgt qe0 qe1 .
+
+Definition qfbv_sge qe0 qe1 := QFBV.Bbinop QFBV.Bsge qe0 qe1 .
+
+Definition qfbv_uaddo qe0 qe1 := QFBV.Bbinop QFBV.Buaddo qe0 qe1 .
+
+Definition qfbv_usubo qe0 qe1 := QFBV.Bbinop QFBV.Busubo qe0 qe1 .
+
+Definition qfbv_umulo qe0 qe1 := QFBV.Bbinop QFBV.Bumulo qe0 qe1 .
+
+Definition qfbv_saddo qe0 qe1 := QFBV.Bbinop QFBV.Bsaddo qe0 qe1 .
+
+Definition qfbv_ssubo qe0 qe1 := QFBV.Bbinop QFBV.Bssubo qe0 qe1 .
+
+Definition qfbv_smulo qe0 qe1 := QFBV.Bbinop QFBV.Bsmulo qe0 qe1 .
+
+Definition qfbv_lneg qb := QFBV.Blneg qb .
+
+Definition qfbv_conj qb0 qb1 := QFBV.Bconj qb0 qb1 .
+
+Definition qfbv_disj qb0 qb1 := QFBV.Bdisj qb0 qb1 .
+
+Definition bexp_instr (te : TypEnv.SSATE.env) (i : SSA.instr) : QFBV.bexp :=
+  match i with
+  (* Inondet (v, t): v = a nondeterministic value of type t *)
+  | SSA.Inondet _ _
+  (* Inop: do nothing *)
+  | SSA.Inop => QFBV.Btrue
+  (* Imov (v, a): v = a *)
+  | SSA.Imov v a =>
+    qfbv_eq (qfbv_var v) (qfbv_atomic a)
+  (* Icmov (v, c, a1, a2): if c then v = a1 else v = a2 *)
+  | SSA.Icmov v c a1 a2 =>
+    let 'qec := qfbv_eq (qfbv_const 1) (qfbv_atomic c) in
+    let 'qe1 := qfbv_atomic a1 in
+    let 'qe2 := qfbv_atomic a2 in
+    qfbv_eq (qfbv_var v) (QFBV.Eite qec qe1 qe2)
+  (* Iadd (v, a1, a2): v = a1 + a2, overflow is forbidden *)
+  | SSA.Iadd v a1 a2 =>
+    let 'qe1 := qfbv_atomic a1 in
+    let 'qe2 := qfbv_atomic a2 in
+    qfbv_eq (qfbv_var v) (qfbv_add qe1 qe2)
+  (* Iadds (c, v, a1, a2): v = a1 + a2, c = carry flag *)
+  | SSA.Iadds c v a1 a2 =>
+    let 'qe1ext := qfbv_zext 1 (qfbv_atomic a1) in
+    let 'qe2ext := qfbv_zext 1 (qfbv_atomic a2) in
+    let 'qerext := qfbv_add qe1ext qe2ext in
+    qfbv_conj
+      (qfbv_eq (qfbv_var c) (qfbv_high 1 qerext))
+      (qfbv_eq (qfbv_var v) (qfbv_low (SSA.asize a1 te) qerext))
+  (* Iadc (v, a1, a2, y): v = a1 + a2 + y, overflow is forbidden *)
+  | SSA.Iadc v a1 a2 y =>
+    let 'qe1 := qfbv_atomic a1 in
+    let 'qe2 := qfbv_atomic a2 in
+    let 'qeyext := qfbv_zext (SSA.asize a1 te - 1) (qfbv_atomic y) in
+    qfbv_eq (qfbv_var v)
+            (qfbv_add (qfbv_add qe1 qe2) qeyext)
+  (* Iadcs (c, v, a1, a2, y): v = a1 + a2 + y, c = carry flag *)
+  | SSA.Iadcs c v a1 a2 y =>
+    let 'qe1ext := qfbv_zext 1 (qfbv_atomic a1) in
+    let 'qe2ext := qfbv_zext 1 (qfbv_atomic a2) in
+    let 'qeyext := qfbv_zext (SSA.asize a1 te) (qfbv_atomic y) in
+    let 'qerext := qfbv_add (qfbv_add qe1ext qe2ext) qeyext in
+    qfbv_conj (qfbv_eq (qfbv_var c) (qfbv_high 1 qerext))
+              (qfbv_eq (qfbv_var v) (qfbv_low (SSA.asize a1 te) qerext))
+  (* Isub (v, a1, a2): v = a1 - a2, overflow is forbidden *)
+  | SSA.Isub v a1 a2 =>
+    let 'qe1 := qfbv_atomic a1 in
+    let 'qe2 := qfbv_atomic a2 in
+    qfbv_eq (qfbv_var v) (qfbv_sub qe1 qe2)
+  (* Isubb (b, v, a1, a2): v = a1 - a2, b = borrow flag *)
+  | SSA.Isubb b v a1 a2 =>
+    let 'qe1ext := qfbv_zext 1 (qfbv_atomic a1) in
+    let 'qe2ext := qfbv_zext 1 (qfbv_atomic a2) in
+    let 'qerext := qfbv_sub qe1ext qe2ext in
+    qfbv_conj (qfbv_eq (qfbv_var b) (qfbv_high 1 qerext))
+              (qfbv_eq (qfbv_var v)
+                       (qfbv_low (SSA.asize a1 te) qerext))
+  (* Isubc (c, v, a1, a2): v = a1 + not(a2) + 1, c = carry flag *)
+  | SSA.Isubc c v a1 a2 =>
+    let 'qe1ext := qfbv_zext 1 (qfbv_atomic a1) in
+    let 'qe2ext := qfbv_zext 1 (qfbv_atomic a2) in
+    let 'qerext := qfbv_sub qe1ext qe2ext in
+    qfbv_conj (qfbv_eq (qfbv_var c)
+                       (qfbv_sub (qfbv_const 1) (qfbv_high 1 qerext)))
+              (qfbv_eq (qfbv_var v)
+                       (qfbv_low (SSA.asize a1 te) qerext))
+  (* Isbb (v, a1, a2, y): v = a1 - a2 - y *)
+  | SSA.Isbb v a1 a2 y =>
+    let 'qe1 := qfbv_atomic a1 in
+    let 'qe2 := qfbv_atomic a2 in
+    let 'qeyext := qfbv_zext (SSA.asize a1 te - 1) (qfbv_atomic y) in
+    qfbv_eq (qfbv_var v) (qfbv_sub (qfbv_sub qe1 qe2) qeyext)
+  (* Isbbs (b, v, a1, a2, y): v = a1 - a2 - y, b = borrow flag *)
+  | SSA.Isbbs b v a1 a2 y =>
+    let 'qe1ext := qfbv_zext 1 (qfbv_atomic a1) in
+    let 'qe2ext := qfbv_zext 1 (qfbv_atomic a2) in
+    let 'qeyext := qfbv_zext (SSA.asize a1 te) (qfbv_atomic y) in
+    let 'qerext := qfbv_sub (qfbv_sub qe1ext qe2ext) qeyext in
+    qfbv_conj (qfbv_eq (qfbv_var b) (qfbv_high 1 qerext))
+              (qfbv_eq (qfbv_var v) (qfbv_low (SSA.asize a1 te) qerext))
+  (* Isbc (v, a1, a2, y): v = a1 + not(a2) + y *)
+  | SSA.Isbc v a1 a2 y =>
+    let 'qe1 := qfbv_atomic a1 in
+    let 'qe2 := qfbv_atomic a2 in
+    let 'qez := qfbv_sub (qfbv_const 1) (qfbv_atomic y) in
+    qfbv_eq (qfbv_var v) (qfbv_sub (qfbv_sub qe1 qe2)
+                                    (qfbv_zext (SSA.asize a1 te - 1) qez))
+  (* Isbcs (c, v, a1, a2, y): v = a1 + not(a2) + y, c = carry flag *)
+  | SSA.Isbcs c v a1 a2 y =>
+    let 'qe1ext := qfbv_zext 1 (qfbv_atomic a1) in
+    let 'qe2ext := qfbv_zext 1 (qfbv_atomic a2) in
+    let 'qez := qfbv_sub (qfbv_const 1) (qfbv_atomic y) in
+    let 'qerext := qfbv_sub (qfbv_sub qe1ext qe2ext)
+                            (qfbv_zext (SSA.asize a1 te) qez) in
+    qfbv_conj (qfbv_eq (qfbv_var c)
+                       (qfbv_sub (qfbv_const 1) (qfbv_high 1 qerext)))
+              (qfbv_eq (qfbv_var v) (qfbv_low (SSA.asize a1 te) qerext))
+  (* Imul (v, a1, a2): v = a1 * a2, overflow is forbidden *)
+  | SSA.Imul v a1 a2 =>
+    let 'qe1 := qfbv_atomic a1 in
+    let 'qe2 := qfbv_atomic a2 in
+    qfbv_eq (qfbv_var v) (qfbv_mul qe1 qe2)
+  (* Imull (vh, vl, a1, a2): vh and vl are respectively the high part and
+     the low part of the full multiplication a1 * a2 *)
+  | SSA.Imull vh vl a1 a2 =>
+    let 'qe1ext := qfbv_zext (SSA.asize a1 te) (qfbv_atomic a1) in
+    let 'qe2ext := qfbv_zext (SSA.asize a1 te) (qfbv_atomic a2) in
+    let 'qerext := qfbv_mul qe1ext qe2ext in
+    qfbv_conj (qfbv_eq (qfbv_var vh)
+                       (qfbv_high (SSA.asize a1 te) qerext))
+              (qfbv_eq (qfbv_var vl)
+                       (qfbv_low (SSA.asize a1 te) qerext))
+  (* Iumulj (v, a1, a2): v = the full multiplication of a1 * a2, which is equivalent
+     to Iumull (vh, vl, a1, a2); Join (r, vh, vl) *)
+  | SSA.Imulj v a1 a2 =>
+    let 'qe1ext := qfbv_zext (SSA.asize a1 te) (qfbv_atomic a1) in
+    let 'qe2ext := qfbv_zext (SSA.asize a1 te) (qfbv_atomic a2) in
+    let 'qerext := qfbv_mul qe1ext qe2ext in
+    qfbv_eq (qfbv_var v) qerext
+  (* Ishl (v, a, n): v = a * 2^n, overflow is forbidden *)
+  (* need a better size for NBitsDef.from_nat *)
+  | SSA.Ishl v a n =>
+    let 'qea := qfbv_atomic a in
+    let 'qen := qfbv_const n in
+    qfbv_eq (qfbv_var v) (qfbv_shl qea qen)
+  (* Ijoin (v, ah, al): v = ah * 2^w + al where w is the bit-width of al *)
+  | SSA.Ijoin v ah al =>
+    let 'qeh := qfbv_atomic ah in
+    let 'qel := qfbv_atomic al in
+    qfbv_eq (qfbv_var v) (qfbv_concat qeh qel)
+  (* Isplit (vh, vl, a, n): vh is the high (w - n) bits (signed extended to w bits)
+     of a and vl is the low n bits (zero extended to w bits) of a where w is the
+     bit-width of a *)
+  | SSA.Isplit vh vl a n =>
+    let 'qea := qfbv_atomic a in
+    let 'qel := qfbv_low n qea in
+    let 'qeh := qfbv_high (SSA.asize a te - n) qea in
+    qfbv_conj (qfbv_eq (qfbv_var vh)
+                       (qfbv_zext (TypEnv.SSATE.vsize vh te - (SSA.asize a te) + n) qeh))
+              (qfbv_eq (qfbv_var vl)
+                       (qfbv_zext (TypEnv.SSATE.vsize vl te - n) qel))
+  (* Icshl (vh, vl, a1, a2, n) *)
+  | SSA.Icshl vh vl a1 a2 n =>
+    let 'qe1 := qfbv_atomic a1 in
+    let 'qe2 := qfbv_atomic a2 in
+    let 'qer := qfbv_shl (qfbv_concat qe1 qe2) (qfbv_const n) in
+    let 'qel := qfbv_low (TypEnv.SSATE.vsize vl te) qer in
+    let 'qeh := qfbv_extr (TypEnv.SSATE.vsize vl te)
+                          (TypEnv.SSATE.vsize vl te + TypEnv.SSATE.vsize vh te - 1) qer in
+    qfbv_conj (qfbv_eq (qfbv_var vh) qeh)
+              (qfbv_eq (qfbv_var vl) qel)
+  (* Inot (v, t, a): v = not(a), the one's complement of a, v is of type t *)
+  | SSA.Inot v t a =>
+    let 'qea := qfbv_atomic a in
+    qfbv_eq (qfbv_var v) qea
+  (* Iand (v, t, a1, a2): v = the bitwise AND of a1 and a2, v is of type t *)
+  | SSA.Iand v t a1 a2 =>
+    let 'qe1 := qfbv_atomic a1 in
+    let 'qe2 := qfbv_atomic a2 in
+    let 'qer := qfbv_and qe1 qe2 in
+    qfbv_eq (qfbv_var v) qer
+  (* Ior (v, t, a1, a2): v = the bitwise OR of a1 and a2, v is of type t *)
+  | SSA.Ior v t a1 a2 =>
+    let 'qe1 := qfbv_atomic a1 in
+    let 'qe2 := qfbv_atomic a2 in
+    let 'qer := qfbv_or qe1 qe2 in
+    qfbv_eq (qfbv_var v) qer
+  (* Ixor (v, t, a1, a2): v = the bitwise XOR of a1 and a2, v is of type t *)
+  | SSA.Ixor v t a1 a2 =>
+    let 'qe1 := qfbv_atomic a1 in
+    let 'qe2 := qfbv_atomic a2 in
+    let 'qer := qfbv_xor qe1 qe2 in
+    qfbv_eq (qfbv_var v) qer
+  (*
+  (* == Instructions that cannot be translated to polynomials == *)
+  (* == Type conversions == *)
+  (* Icast (v, t, a): v = the value of a represented by the type t of v *)
+  | SSA.Icast v t a
+  (* Ivpc (v, t, a): v = a, value preserved casting to type t *)
+  | SSA.Ivpc v t a
+  (* Specifications *)
+  | SSA.Iassume : bexp -> instr
+ *)
+  | _ => QFBV.Bfalse
+  end .
+
+Definition bexp_program te (p : program) : seq QFBV.bexp :=
+  map (bexp_instr te) p.
+
+Fixpoint exp_rexp (e : SSA.rexp) : QFBV.exp :=
+  match e with
+  | Rvar v => qfbv_var v
+  | Rconst _ n => QFBV.Econst n
+  | Runop w op e =>
+    match op with
+    | Rnegb => qfbv_neg (exp_rexp e)
+    | Rnotb => qfbv_not (exp_rexp e)
+    end
+  | Rbinop _ op e1 e2 =>
+    match op with
+    | Radd => qfbv_add (exp_rexp e1) (exp_rexp e2)
+    | Rsub => qfbv_sub (exp_rexp e1) (exp_rexp e2)
+    | Rmul => qfbv_mul (exp_rexp e1) (exp_rexp e2)
+    | Rumod => qfbv_mod (exp_rexp e1) (exp_rexp e2)
+    | Rsrem => qfbv_srem (exp_rexp e1) (exp_rexp e2)
+    | Rsmod => qfbv_smod (exp_rexp e1) (exp_rexp e2)
+    | Randb => qfbv_and (exp_rexp e1) (exp_rexp e2)
+    | Rorb => qfbv_or (exp_rexp e1) (exp_rexp e2)
+    | Rxorb => qfbv_xor (exp_rexp e1) (exp_rexp e2)
+    end
+  | Ruext _ e n => qfbv_zext n (exp_rexp e)
+  | Rsext _ e n => qfbv_sext n (exp_rexp e)
+  end .
+
+Fixpoint bexp_rbexp (e : SSA.rbexp) : QFBV.bexp :=
+  match e with
+  | Rtrue => QFBV.Btrue
+  | Req _ e1 e2 =>
+    qfbv_eq (exp_rexp e1) (exp_rexp e2)
+  | Rcmp _ op e1 e2 =>
+    match op with
+    | Rult => qfbv_ult (exp_rexp e1) (exp_rexp e2)
+    | Rule => qfbv_ule (exp_rexp e1) (exp_rexp e2)
+    | Rugt => qfbv_ugt (exp_rexp e1) (exp_rexp e2)
+    | Ruge => qfbv_uge (exp_rexp e1) (exp_rexp e2)
+    | Rslt => qfbv_slt (exp_rexp e1) (exp_rexp e2)
+    | Rsle => qfbv_sle (exp_rexp e1) (exp_rexp e2)
+    | Rsgt => qfbv_sgt (exp_rexp e1) (exp_rexp e2)
+    | Rsge => qfbv_sge (exp_rexp e1) (exp_rexp e2)
+    end 
+  | Rneg e => qfbv_lneg (bexp_rbexp e)
+  | Rand e1 e2 =>
+    qfbv_conj (bexp_rbexp e1) (bexp_rbexp e2)
+  | Ror e1 e2 =>
+    qfbv_disj (bexp_rbexp e1) (bexp_rbexp e2)
+  end .
+
+Record bexp_spec : Type :=
+  mkQFBVSpec { bpre : QFBV.bexp;
+               bprog : seq QFBV.bexp;
+               bpost : QFBV.bexp } .
+
+Definition bexp_of_rspec te (s : rspec) : bexp_spec :=
+  {| bpre := bexp_rbexp (rspre s);
+     bprog := bexp_program te (rsprog s);
+     bpost := bexp_rbexp (rspost s) |}.
+
+(* properties of conversion *)
+
+Lemma eval_exp_var v s :
+  QFBV.eval_exp (qfbv_var v) s = SSAStore.acc v s.
+Proof.
+  reflexivity.
+Qed.
+
+Lemma eval_exp_atomic a s :
+  QFBV.eval_exp (qfbv_atomic a) s = eval_atomic a s.
+Proof.
+  case: a => /=; reflexivity.
+Qed.
+
+Lemma eval_exp_rexp (e : SSA.rexp) s:
+  QFBV.eval_exp (exp_rexp e) s = eval_rexp e s.
+Admitted .
+(* TODO: wait for the mod, smod, srem
+Proof .
+  elim: e => /=.
+  - reflexivity.
+  - reflexivity.
+  - move=> w op e IH;
+             case : op; rewrite /= IH; reflexivity .
+  - move=> w op e0 IH0 e1 IH1 .
+    case : op; rewrite /=; rewrite IH0 IH1 // .
+  - move => w e IH n; rewrite /= IH // .
+  - move => w e IH n; rewrite /= IH // .
+    
+Qed.
+ *)
+
+Lemma eval_bexp_rbexp e s:
+  QFBV.eval_bexp (bexp_rbexp e) s <-> eval_rbexp e s .
+Proof .
+  elim : e => /= .
+  - done .
+  - move => w e0 e1; split .
+    + move => /eqP Heq; rewrite -!eval_exp_rexp Heq // .
+    + move => Heq; rewrite !eval_exp_rexp Heq // .
+  - move => w op e0 e1;
+      elim : op => /=; rewrite -!eval_exp_rexp // .
+  - move => e; elim => Hleft Hright; split .
+    + move => /negP Hneg .
+      red; move => Heval .
+      move : (Hright Heval); done .
+    + move => Heval .
+      apply /negP; red; move => Hneg .
+      move : (Hleft Hneg); done .
+  - move => e0 IH0 e1 IH1; split .
+    + move => /andP [Heval0 Heval1] .
+      tauto .
+    + move => [Heval0 Heval1] .
+      elim IH0 => {IH0} _ IH0; elim IH1 => {IH1} _ IH1 .
+      rewrite (IH0 Heval0) (IH1 Heval1) // .
+  - move => e0 IH0 e1 IH1; split .
+    + move => /orP Hor .
+      tauto .
+    + move => Hor .
+      elim IH0 => {IH0} _ IH0; elim IH1 => {IH1} _ IH1 .
+      elim Hor; move => He; apply /orP; tauto .
+Qed .
+
+Lemma eval_bexp_rbexp1 e s:
+  QFBV.eval_bexp (bexp_rbexp e) s -> eval_rbexp e s.
+Proof.
+  move: (eval_bexp_rbexp e s) => [H1 H2]. exact: H1.
+Qed.
+
+Lemma eval_bexp_rbexp2 e s:
+  eval_rbexp e s -> QFBV.eval_bexp (bexp_rbexp e) s.
+Proof.
+  move: (eval_bexp_rbexp e s) => [H1 H2]. exact: H2.
+Qed.
 
 (* Define the safety condition in terms of a QFBV expression *)
 (* TODO: see bexp_program_safe in certified_qhasm_vcg/mqhasm/bvSSA2QFBV.v *)
 Definition bexp_program_safe (p : program) : QFBV.bexp := QFBV.Btrue.
+
+
